Libraries slightly enhanced

OkLib.v
@@ -7,39 +7,151 @@ Require Export LibVar.
 Require Export LibList.
 Require Import Setoid.
 
-Require Import LibTactics. (* for skip *)
+Require Export LibTactics. (* for skip *)
 
 Open Scope permut_scope.
 
 (*** Definitions ***)
+Set Implicit Arguments.
 
-Fixpoint ok A (G: list (var * A)) (Used: list var) : Prop :=
-match G with 
+Section Definitions.
+
+Variable A: Type.
+
+Fixpoint ok (G: list (var * A)) (Used: list var) : Prop :=
+match G with
 | nil => True
-| (w, Gamma) :: G => If Mem w Used then False else ok A G (w::Used)
+| (w, Gamma) :: G => If Mem w Used then False else ok G (w::Used)
 end.
 
+End Definitions.
+
 Definition ok_Bg (G: Background_LF) : Prop :=
-ok (list (var * ty)) G nil  /\
-ok (ty) (flat_map snd G) nil.
+ok G nil  /\
+ok (flat_map snd G) nil.
 
 Fixpoint used_t_vars (G: Background_LF) :=
 match G with
 | nil => from_list nil
 | (w, Gamma) :: G => from_list (map fst Gamma) \u used_t_vars G
-end. 
+end.
 
 Fixpoint used_w_vars (G: Background_LF) :=
 match G with
 | nil => from_list nil
 | (w, Gamma) :: G => \{w} \u used_w_vars G
-end. 
+end.
 
 (*** Lemmas ***)
 
-(* FIXME: Admitted *)
+(* ok for a generic type *)
+
+Lemma ok_used_permut:
+forall A G U U',
+  U *=* U' ->
+  (@ok A G U) ->
+  (@ok A G U').
+induction G; intros; simpl in *; auto.
+destruct a; repeat case_if.
+elim H2; apply Mem_permut with (l:=U'); [ symmetry | ]; auto.
+eapply IHG; eauto.
+Qed.
+
+Lemma ok_used_weakening:
+forall A G x U,
+  (@ok A G (x::U)) ->
+  (@ok A G U).
+induction G; simpl; intros; auto;
+destruct a; repeat case_if.
+elim H1; rewrite Mem_cons_eq; right; auto.
+apply IHG with (x:=x).
+apply ok_used_permut with (U := (v::x::U));
+[ permut_simpl | auto].
+Qed.
+
+Lemma ok_split:
+forall A G1 G2 U,
+  (@ok A (G1++G2) U) ->
+  ok G1 U /\ ok G2 U.
+induction G1; intros; split; rew_app in *; simpl; auto;
+destruct a; simpl in *; case_if.
+apply IHG1 with (G2:=G2); eauto.
+apply IHG1 with (G2:=G2); apply ok_used_weakening in H; eauto.
+Qed.
+
+(* ok for a specific type -- would be nice to make it more general btw *)
+
+Add Morphism (@ok (list (var*ty))) : ok_PPermut_lst_var_ty.
+Admitted. (* !!! *)
+
+(* FIXME: how to add this as morphism? *)
+Lemma ok_PPermut_ty:
+forall G G', G ~=~ G' ->
+  ok (flat_map snd G) nil ->
+  ok (flat_map snd G') nil.
+Admitted. (* !!! *)
+
+Lemma ok_fresh_te_list:
+forall G Gamma v A w,
+ ok ((w, Gamma) :: G) nil ->
+ v \notin (used_t_vars ((w,Gamma)::G)) ->
+ ok ((w, (v,A)::Gamma) :: G) nil.
+Admitted. (* !!! *)
+
+Lemma ok_fresh_te_ty:
+forall G Gamma v A w,
+ ok (flat_map snd ((w, Gamma) :: G)) nil ->
+ v \notin (used_t_vars ((w,Gamma)::G)) ->
+ ok (flat_map snd ((w, (v,A)::Gamma) :: G)) nil.
+Admitted. (* !!! *)
+
+Lemma ok_fresh_wo_list:
+forall G v w,
+ ok G nil ->
+ v \notin (used_w_vars G) ->
+ ok ((w, nil) :: G) nil.
+Admitted. (* !!! *)
+
+Lemma ok_fresh_wo_ty:
+forall G v w,
+ ok (flat_map snd G) nil ->
+ v \notin (used_w_vars G) ->
+ ok (flat_map snd ((w, nil) :: G)) nil.
+Admitted. (* !!! *)
+
+Lemma ok_fresh_wo_te_list:
+forall G v A w,
+ ok G nil ->
+ w \notin (used_w_vars G) ->
+ ok ((w, (v,A)::nil) :: G) nil.
+Admitted. (* !!! *)
+
+Lemma ok_fresh_wo_te_ty:
+forall G v A w,
+ ok (flat_map snd G) nil ->
+ w \notin (used_w_vars G) ->
+ ok (flat_map snd ((w, (v,A)::nil) :: G)) nil.
+Admitted. (* !!! *)
+
+Lemma ok_empty_first_list:
+forall w G Gamma,
+  ok ((w,Gamma) :: G) nil ->
+  ok ((w, (@nil (prod var ty))) :: G) nil.
+Admitted. (* !!! *)
+
+Lemma ok_empty_first_ty:
+forall (w: var) G Gamma,
+  (@ok ty (flat_map snd ((w,Gamma) :: G)) nil) ->
+  (@ok ty (flat_map snd ((w, nil) :: G)) nil).
+Admitted. (* !!! *)
+
+(* ok_Bg *)
+
 Add Morphism ok_Bg : ok_Bg_PPermut.
-skip.
+intros; unfold ok_Bg; split; intros;
+destruct H0; split;
+[ rewrite <- H | eapply ok_PPermut_ty |
+  rewrite H | eapply ok_PPermut_ty; try symmetry ]; eauto.
 Qed.
 
 Lemma ok_Bg_ppermut:
@@ -50,58 +162,73 @@ forall G G',
 intros; rewrite <- H; auto.
 Qed.
 
-(* FIXME: Admitted *)
 Lemma ok_Bg_permut:
 forall G Ctx Ctx' w,
   Ctx *=* Ctx' ->
   ok_Bg ((w, Ctx) :: G) ->
   ok_Bg ((w, Ctx') :: G).
-Admitted.
+intros;
+assert ((w, Ctx) :: G ~=~ (w, Ctx') :: G) by PPermut_simpl;
+rewrite <- H1; auto.
+Qed.
 
-(* FIXME: Admitted *)
 Lemma ok_Bg_permut_last:
 forall G Ctx Ctx' w,
   Ctx *=* Ctx' ->
   ok_Bg (G ++ (w, Ctx) :: nil) ->
   ok_Bg (G ++ (w, Ctx') :: nil).
-Admitted.
+intros;
+assert (G & (w, Ctx) ~=~ G & (w, Ctx')) by PPermut_simpl;
+rewrite <- H1; auto.
+Qed.
 
-(* FIXME: Admitted *)
 Lemma ok_Bg_fresh_te:
 forall G Gamma v A w,
  ok_Bg ((w, Gamma) :: G) ->
  v \notin (used_t_vars ((w,Gamma)::G)) ->
  ok_Bg ((w, (v,A)::Gamma) :: G).
-Admitted.
+intros; unfold ok_Bg in *;  destruct H; split;
+[ apply ok_fresh_te_list |
+  apply ok_fresh_te_ty]; auto.
+Qed.
 
-(* FIXME: Admitted *)
 Lemma ok_Bg_fresh_wo:
 forall G w,
  ok_Bg G ->
  w \notin (used_w_vars G) ->
  ok_Bg ((w, nil) :: G).
-Admitted.
+intros; unfold ok_Bg in *;  destruct H; split;
+[ eapply ok_fresh_wo_list |
+  eapply ok_fresh_wo_ty]; eauto.
+Qed.
 
-(* FIXME: Admitted *)
 Lemma ok_Bg_fresh_wo_te:
 forall G w v A,
  ok_Bg G ->
  w \notin (used_w_vars G) ->
  ok_Bg ((w, (v, A) :: nil) :: G).
-Admitted.
+intros; unfold ok_Bg in *;  destruct H; split;
+[ apply ok_fresh_wo_te_list |
+  apply ok_fresh_wo_te_ty]; eauto.
+Qed.
 
 Lemma ok_Bg_cons_last:
 forall G a,
   ok_Bg (G & a) <-> ok_Bg (a :: G).
-Admitted.
+intros; assert (G & a ~=~ a :: G) by PPermut_simpl;
+rewrite H; split; auto.
+Qed.
 
 Lemma ok_Bg_swap:
 forall C C' G,
   ok_Bg (C :: G & C') ->
   ok_Bg (C' :: G & C).
-Admitted.
+intros; assert (C:: G & C' ~=~ C' :: G & C) by PPermut_simpl;
+rewrite <- H0; auto.
+Qed.
 
-Hint Resolve ok_Bg_cons_last ok_Bg_swap ok_Bg_permut_last.
+Hint Resolve ok_Bg_cons_last ok_Bg_swap.
+Hint Resolve ok_Bg_permut_last: ok_bg_rew.
 Hint Resolve ok_Bg_fresh_te ok_Bg_fresh_wo ok_Bg_fresh_wo_te.
 
 Lemma ok_Bg_permut_first_tail:
@@ -109,16 +236,24 @@ forall G C C' w x A,
   ok_Bg ((w, C) :: G) ->
   C *=* (x,A)::C' ->
   ok_Bg ((w, C') :: G).
-Admitted.
-Hint Resolve ok_Bg_permut_first_tail.
+intros;
+assert ((w,(x, A) :: C') :: G ~=~ (w, C) :: G) by PPermut_simpl;
+rewrite <- H1 in H; unfold ok_Bg in *; destruct H; split; simpl in *;
+repeat case_if; auto;
+apply ok_used_weakening with (x:=x); auto.
+Qed.
+Hint Resolve ok_Bg_permut_first_tail : ok_bg_rew.
 
 Lemma ok_Bg_empty_first:
 forall w G Gamma,
   ok_Bg ((w,Gamma) :: G) ->
   ok_Bg ((w, nil) :: G).
-Admitted.
+intros; unfold ok_Bg; destruct H; split;
+[eapply ok_empty_first_list |
+ eapply ok_empty_first_ty]; eauto.
+Qed.
 
-Hint Resolve ok_Bg_empty_first.
+Hint Resolve ok_Bg_empty_first : ok_bg_rew.
 
 Lemma ok_Bg_Mem_eq:
 forall w C C' v A A0 G,
@@ -126,7 +261,18 @@ forall w C C' v A A0 G,
   C *=* (v, A) :: C' ->
   Mem (v, A0) C ->
   A0 = A.
-Admitted.
+intros; destruct (eq_ty_dec A0 A); auto;
+assert (exists gh, exists gt, C' = gh & (v, A0) ++ gt) by
+  ( apply permut_neq_split with (b := (v, A)) (l1 := C); auto;
+    intro HH; inversion HH; subst; elim n; auto);
+destruct H2 as (gh); destruct H2 as (gt); subst;
+assert (C *=* (v, A) :: (v, A0) :: gh ++ gt) by (rewrite H0; permut_simpl);
+unfold ok_Bg in *; destruct H;
+assert (ok (flat_map snd ((w, (v, A) :: (v, A0) :: gh ++ gt ) :: G )) nil) by
+  (apply ok_PPermut_ty with (G := ((w, C) :: G)); [PPermut_simpl | auto]);
+simpl in *; repeat case_if;
+elim H6; apply Mem_here.
+Qed.
 
 Lemma ok_Bg_Mem_contradict:
 forall A A' w w' v C C' G G',
@@ -134,50 +280,101 @@ forall A A' w w' v C C' G G',
  Mem (v, A) C ->
  G ~=~ G' & (w', (v, A') :: C') ->
  False.
-Admitted.
+intros.
+rewrite H1 in H.
+apply permut_Mem_split_head with (l2 := C) in H0; auto;
+destruct H0 as (gh); destruct H0 as (gt); subst.
+assert ((w, gh & (v, A) ++ gt) :: G' & (w', (v, A') :: C') ~=~
+        (w, (v, A) :: gh ++ gt) :: (w', (v, A') :: C') :: G') by
+(PPermut_simpl; apply PPermut_skip; [permut_simpl | auto]).
+rewrite H0 in H; unfold ok_Bg in H; destruct H.
+simpl in *; repeat case_if.
+assert (ok ((v, A') :: C' ++ flat_map snd G') (v :: nil)).
+  eapply ok_split with (G1:=gh++gt). (* exact H2.  ?!? *) skip. (* !!! *)
+simpl in H6; case_if; elim H7; apply Mem_here.
+Qed.
 
 Lemma ok_Bg_permut_no_last:
 forall G w C v A,
   ok_Bg (G & (w, (v,A) :: C)) ->
   ok_Bg (G & (w, C)).
-Admitted.
+Admitted. (* !!! *)
 
 Lemma ok_Bg_permut_no_last_spec:
 forall G w C C0 v A,
   ok_Bg (C0::G & (w, (v,A) :: C)) ->
   ok_Bg (C0::G & (w, C)).
-Admitted.
+intros;
+assert (C0 :: G & (w, C)  ~=~ (C0 :: G) & (w, C)) by (rew_app; PPermut_simpl);
+rewrite H0; eapply ok_Bg_permut_no_last; rew_app; eauto.
+Qed.
 
 Lemma ok_Bg_no_last:
 forall G w C,
   ok_Bg (G & (w,C)) ->
   ok_Bg G.
-Admitted.
+intros. assert (G & (w,C) ~=~ ((w, C) :: nil) ++ G) by PPermut_simpl;
+rewrite H0 in H;
+destruct H; split.
+eapply ok_split in H; destruct H; auto.
+simpl in H1.
+assert (ok C nil /\ ok (flat_map snd G) nil) by skip. (* !!! *)
+  (* eapply ok_split with (A:= var) (G1:=C) (G2:=flat_map snd G) (U:=nil). *)
+destruct H2; auto.
+Qed.
 Hint Resolve ok_Bg_no_last.
 
 Lemma ok_Bg_permut_no_last_spec2:
 forall G w C C0 v A,
   ok_Bg (G & (w, (v,A) :: C) & C0) ->
   ok_Bg (G & (w, C) & C0).
-Admitted.
+intros.
+assert (G & (w, C) & C0 ~=~ G & C0 & (w, C)) by PPermut_simpl;
+rewrite H0;
+apply ok_Bg_permut_no_last with (v:=v) (A:=A).
+assert (G & C0 & (w, (v, A) :: C) ~=~ G & (w, (v, A) :: C) & C0)
+  by PPermut_simpl;
+rewrite H1; auto.
+Qed.
 
 Lemma ok_Bg_first_last_neq:
 forall w w' C C' G,
   ok_Bg ((w, C) :: G & (w', C')) ->
   w <> w'.
-Admitted.
+intros.
+assert ((w, C) :: G & (w', C') ~=~ (w, C) :: (w', C') :: G) by PPermut_simpl;
+rewrite H0 in H;
+destruct H; simpl in *; repeat case_if.
+intro; elim H3; rewrite Mem_cons_eq; left; symmetry; auto.
+Qed.
 
 Lemma ok_Bg_last_last2_neq:
 forall w w' C C' G,
   ok_Bg (G & (w, C) & (w', C')) ->
   w <> w'.
-Admitted.
+intros;
+assert (G & (w, C) & (w', C') ~=~ (w, C) :: (w', C') :: G) by PPermut_simpl;
+rewrite H0 in H;
+destruct H; simpl in *; repeat case_if.
+intro; elim H3; rewrite Mem_cons_eq; left; symmetry; auto.
+Qed.
 
 Lemma ok_Bg_swap_worlds:
 forall G w w' C C',
   ok_Bg (G & (w, C) & (w', C')) ->
   ok_Bg (G & (w', C) & (w, C')).
-Admitted.
+intros.
+assert (G & (w, C) & (w', C') ~=~ (w, C) :: (w', C') :: G) by PPermut_simpl.
+rewrite H0 in H.
+assert (G & (w', C) & (w, C') ~=~ (w', C) :: (w, C') :: G) by PPermut_simpl.
+rewrite H1.
+destruct H; split; simpl in *; repeat case_if.
+rewrite Mem_nil_eq in H3; auto.
+rewrite Mem_cons_eq in H4; elim H6; destruct H4; subst;
+[ apply Mem_here | rewrite Mem_nil_eq in H4; contradiction].
+apply ok_used_permut with (U := w'::w::nil); [permut_simpl | ]; auto.
+auto.
+Qed.
 
 Lemma ok_Bg_impl_ppermut:
 forall G G' w C C',
@@ -186,73 +383,199 @@ forall G G' w C C',
   G ~=~ G' /\ C *=* C'.
 Admitted.
 
+
+(* FIXME: generalize all the ok_Bg_split* into :
+   ok_Bg G <- ok_Bg reorder_G <- ok_Bg reorder_G' <- ok_Bg G':
+   reorder X ~=~ X and all the singletons are in the front *)
+
+
 Lemma ok_Bg_split1:
 forall G w w' C C',
   ok_Bg ((w,C)::G & (w',C')) ->
   ok_Bg ((w, C ++ C') :: G).
-Admitted.
+intros.
+assert ((w, C) :: G & (w', C') ~=~ (w,C) :: (w', C')::G) by PPermut_simpl.
+rewrite H0 in H; destruct H; split; simpl in *;
+repeat case_if.
+apply ok_used_weakening with (x:=w'); auto.
+skip. (* this should be rew_app; auto *)
+Qed.
 
 Lemma ok_Bg_split2:
 forall G w w' C C',
   ok_Bg ((w,C)::G & (w',C')) ->
   ok_Bg ((w', C' ++ C) :: G).
-Admitted.
+intros.
+assert ((w, C) :: G & (w', C') ~=~ (w', C') :: (w, C)::G) by PPermut_simpl.
+rewrite H0 in H; destruct H; split; simpl in *;
+repeat case_if.
+rewrite Mem_nil_eq in H2; auto.
+apply ok_used_weakening with (x:=w); auto.
+skip. (* this should be rew_app; auto *)
+Qed.
 
 Lemma ok_Bg_split3:
 forall G w w' w'' C C' C'',
   ok_Bg ((w,C)::G & (w',C') & (w'',C'')) ->
   ok_Bg ((w, C) :: G & (w', C' ++ C'')).
-Admitted.
+intros.
+assert ((w, C) :: G & (w', C') & (w'',C'') ~=~
+  (w, C) :: (w', C'):: (w'',C'') :: G) by PPermut_simpl.
+assert ((w,C) :: G & (w', C'++C'') ~=~ (w,C) :: (w', C'++C'') :: G)
+  by PPermut_simpl.
+rewrite H0 in H; rewrite H1; destruct H; split; simpl in *;
+repeat case_if.
+apply ok_used_weakening with (x:=w''); auto.
+skip. (* this should be rew_app; auto *)
+Qed.
 
 Lemma ok_Bg_split4:
 forall G w w' C C',
   ok_Bg (G & (w, C) & (w', C')) ->
   ok_Bg (G & (w', C' ++ C)).
-Admitted.
+intros.
+assert (G & (w, C) & (w', C') ~=~
+  (w, C) :: (w', C') :: G) by PPermut_simpl.
+assert (G & (w', C'++C) ~=~ (w', C'++C) :: G)
+  by PPermut_simpl.
+rewrite H0 in H; rewrite H1; destruct H; split; simpl in *;
+repeat case_if.
+rewrite Mem_nil_eq in H3; auto.
+apply ok_used_weakening with (x:=w);
+apply ok_used_permut with (U:= w'::w::nil).
+permut_simpl. auto.
+skip. (* this should be rew_app; auto *)
+Qed.
 
 Lemma ok_Bg_split5:
 forall G w w' C C',
   ok_Bg (G & (w, C) & (w', C')) ->
   ok_Bg (G & (w, C ++ C')).
-Admitted.
+intros.
+assert (G & (w, C) & (w', C') ~=~
+  (w, C) :: (w', C') :: G) by PPermut_simpl.
+assert (G & (w, C++C') ~=~ (w, C++C') :: G)
+  by PPermut_simpl.
+rewrite H0 in H; rewrite H1; destruct H; split; simpl in *;
+repeat case_if.
+apply ok_used_weakening with (x:=w'); auto.
+skip. (* this should be rew_app; auto *)
+Qed.
 
 Lemma ok_Bg_split6:
 forall G w C C' C'' w' w'',
   ok_Bg (G & (w, C) & (w', C') & (w'', C'')) ->
   ok_Bg (G & (w, C ++ C') & (w'', C'')).
-Admitted.
+intros.
+assert (G & (w,C) & (w', C') & (w'',C'') ~=~
+  (w, C) :: (w', C'):: (w'',C'') :: G) by PPermut_simpl.
+assert (G & (w, C++C') & (w'', C'') ~=~ (w, C ++ C') :: (w'', C'') :: G)
+  by PPermut_simpl.
+rewrite H0 in H; rewrite H1; destruct H; split; simpl in *;
+repeat case_if.
+rewrite Mem_cons_eq in H4;destruct H4; subst.
+elim H6; rewrite Mem_cons_eq; right; apply Mem_here.
+rewrite Mem_nil_eq in H4; auto.
+apply ok_used_weakening with (x:=w');
+apply ok_used_permut with (U:= w''::w'::w::nil).
+  permut_simpl.
+  auto.
+skip. (* this should be rew_app; auto *)
+Qed.
 
+(* This is actually false
 Lemma ok_Bg_split7:
 forall G w w' w'' C C' C'',
   ok_Bg ((w,C)::G & (w'',C'')) ->
   ok_Bg ((w, C ++ C'') :: G & (w', C')).
-Admitted.
+*)
 
 Lemma ok_Bg_split8:
 forall G G' w w' w'' C C' C'',
   ok_Bg (G ++ G' ++ (w, C) :: (w', C') :: (w'', C'') :: nil) ->
   ok_Bg (G ++ G' ++ (w', C') :: (w'', C'' ++ C)::nil) .
-Admitted.
+intros.
+assert (G++G' ++ (w, C) :: (w', C') :: (w'',C'') :: nil ~=~
+  (w, C) :: (w', C'):: (w'',C'') :: G ++ G') by PPermut_simpl.
+assert (G ++ G' ++ (w', C') :: (w'', C'' ++ C) :: nil ~=~
+  (w', C') :: (w'', C''++C) :: G ++ G')
+  by PPermut_simpl.
+rewrite H0 in H; rewrite H1; destruct H; split; simpl in *;
+repeat case_if.
+rewrite Mem_nil_eq in H3; auto.
+rewrite Mem_cons_eq in H4; destruct H4; subst.
+elim H7; rewrite Mem_cons_eq; left; auto.
+rewrite Mem_nil_eq in H4; auto.
+apply ok_used_weakening with (x:=w);
+apply ok_used_permut with (U:=w'' :: w' :: w :: nil);
+auto; permut_simpl.
+skip. (* this should be rew_app; permut; auto *)
+Qed.
 
 Lemma ok_Bg_split9:
 forall G w w' w'' C C' C'',
   ok_Bg ((w,C)::G & (w',C') & (w'',C'')) ->
   ok_Bg ((w, C++C') :: G & (w'', C'')).
-Admitted.
+intros.
+assert ((w, C) :: G & (w', C') & (w'',C'') ~=~
+  (w, C) :: (w', C'):: (w'',C'') :: G) by PPermut_simpl.
+assert ((w, C++C') :: G & (w'', C'')  ~=~
+  (w, C++C') :: (w'', C'') :: G)
+  by PPermut_simpl.
+rewrite H0 in H; rewrite H1; destruct H; split; simpl in *;
+repeat case_if.
+rewrite Mem_cons_eq in H4; destruct H4; subst.
+elim H6; rewrite Mem_cons_eq; right; apply Mem_here.
+rewrite Mem_nil_eq in H4; auto.
+apply ok_used_weakening with (x:=w');
+apply ok_used_permut with (U:=w'' :: w' :: w :: nil);
+auto; permut_simpl.
+skip. (* this should be rew_app; permut; auto *)
+Qed.
 
 Lemma ok_Bg_split10:
 forall G G' w1 w2 w3 w4 c1 c2 c3 c4,
   ok_Bg (G ++ (w1, c1)::G' ++ (w2, c2) :: (w3, c3) :: (w4, c4) :: nil) ->
   ok_Bg (G ++ (w1, c1)::G' ++ (w2, c2 ++ c3) :: (w4, c4) :: nil).
-Admitted.
+intros.
+assert (G ++ (w1,c1) :: G' ++ (w2, c2) :: (w3, c3) :: (w4,c4) :: nil ~=~
+   (w1,c1) :: (w2, c2) :: (w3, c3) :: (w4,c4) :: G ++ G') by PPermut_simpl.
+assert (G ++ (w1, c1) :: G' ++ (w2, c2 ++ c3) :: (w4, c4) :: nil~=~
+   (w1,c1) :: (w2, c2 ++ c3) :: (w4,c4) :: G ++ G') by PPermut_simpl.
+rewrite H0 in H; rewrite H1; destruct H; split; simpl in *;
+repeat case_if.
+rewrite Mem_cons_eq in H5. destruct H5; subst.
+elim H7; rewrite Mem_cons_eq; right; apply Mem_here.
+rewrite Mem_cons_eq in H5. destruct H5; subst.
+elim H7; rewrite Mem_cons_eq; right;
+rewrite Mem_cons_eq; right; apply Mem_here.
+rewrite Mem_nil_eq in H5; auto.
+apply ok_used_weakening with (x:=w3);
+apply ok_used_permut with (U:=w4 :: w3 :: w2 :: w1 :: nil);
+auto; permut_simpl.
+skip. (* this should be rew_app; permut; auto *)
+Qed.
 
-Hint Resolve ok_Bg_split1 ok_Bg_split2 ok_Bg_split3 ok_Bg_split4 ok_Bg_split5 ok_Bg_split6 ok_Bg_split7 ok_Bg_split8 ok_Bg_split9 ok_Bg_split10.
-Hint Resolve ok_Bg_permut_no_last ok_Bg_permut_no_last_spec2 ok_Bg_permut_no_last_spec ok_Bg_first_last_neq ok_Bg_last_last2_neq ok_Bg_swap_worlds. 
+Hint Resolve ok_Bg_split1 ok_Bg_split2 ok_Bg_split3 ok_Bg_split4
+  ok_Bg_split5 ok_Bg_split6 ok_Bg_split8
+  ok_Bg_split9 ok_Bg_split10 : ok_bg_rew.
+Hint Resolve ok_Bg_permut_no_last ok_Bg_permut_no_last_spec2
+  ok_Bg_permut_no_last_spec ok_Bg_first_last_neq
+  ok_Bg_last_last2_neq : ok_bg_rew.
+Hint Resolve ok_Bg_swap_worlds.
 
 Lemma ok_Bg_skip_last:
 forall G C,
   ok_Bg (G & C) -> ok_Bg G.
-Admitted.
+intros;
+assert (G & C ~=~ (C :: nil) ++ G) by PPermut_simpl; rewrite H0 in H;
+destruct H; split.
+eapply ok_split with (G1:=C::nil) (G2:=G); eauto.
+simpl in *; destruct C; case_if.
+eapply ok_split with (G1:=snd (v,l)) (G2:=flat_map snd  G); auto.
+skip. (* exact H1 *)
+Qed.
 
+Hint Resolve ok_Bg_skip_last: ok_bg_rew.
 
 Close Scope permut_scope.
